src/Bedrock.v
@@ -1,5 +1,5 @@
 Require Export String List.
 
-Require Export Nomega Word IL LabelMap PropX PropXTac XCAP Structured StructuredModule Programming.
+Require Export Nomega Word IL LabelMap PropX PropXTac XCAP Structured StructuredModule Linker Programming.
 
 Open Scope string_scope.
